Completely updated libraries

pulse/ulib/LowStar.RST.Array.Loops.fst
@@ -17,24 +17,31 @@ open FStar.Mul
 
 let iteri #a b context loop_inv f len =
   (**) let hinit = HST.get () in
-  (**) assume(RST.rst_inv (AR.array_resource b) hinit);
-  (**) let init = RST.get (R.(AR.array_resource b <*> context)) in
-  (**) let correct_inv = fun (b_view, context_view) i -> loop_inv context_view i /\
-  (**)  init (AR.array_resource b) == b_view
-  (**) in
   (**) R.reveal_star ();
+  (**) RST.reveal_rst_inv ();
+  (**) let init = RST.get (R.(AR.array_resource b <*> context)) in
+  (**) let correct_inv (sel : RST.selector ((R.(AR.array_resource b <*> context)))) (i : nat) =
+  (**)  loop_inv (RST.focus_selector sel context) i /\
+  (**)  init (AR.array_resource b) == (sel (AR.array_resource b))
+  (**) in
   let correct_f (i:U32.t{U32.(0 <= v i /\ v i < A.vlength b)})
     : RST.RST unit
       (R.(AR.array_resource b <*> context))
       (fun _ -> R.(AR.array_resource b <*> context))
       (requires (fun old ->
-        correct_inv (old (R.(AR.array_resource b <*> context))) (U32.v i)
+        correct_inv old (U32.v i)
       ))
       (ensures (fun old _ modern -> U32.(
-        correct_inv (old R.(AR.array_resource b <*> context)) (v i) /\
-        correct_inv (modern R.(AR.array_resource b <*> context)) (v i + 1)
+        correct_inv old (v i) /\
+        correct_inv modern (v i + 1)
       )))
   =
+    let old = RST.get (R.(AR.array_resource b <*> context)) in
+    assume(loop_inv (RST.focus_selector old context) (U32.v i));
+    assume(init (AR.array_resource b) == (old (AR.array_resource b)));
+    assert(correct_inv old (U32.v i));
+    admit();
+    let h0 = HST.get () in
     let x = RST.rst_frame
       (R.(AR.array_resource b <*> context))
       (fun _ -> R.(AR.array_resource b <*> context))
@@ -43,18 +50,16 @@ let iteri #a b context loop_inv f len =
     let f' () : RST.RST unit // TODO: figure out why we cannot remove this superfluous let-binding
       (context)
       (fun _ -> context)
-      (fun old ->  loop_inv (old context) (U32.v i))
-      (fun old _ modern -> loop_inv (old context) (U32.v i) /\ loop_inv (modern context) (U32.v i + 1))
+      (fun old -> loop_inv old (U32.v i))
+      (fun old _ modern -> loop_inv old (U32.v i) /\ loop_inv modern (U32.v i + 1))
       =
       f i x
     in
-     RST.rst_frame
-       R.(AR.array_resource b <*> context)
-       (fun _ -> R.(AR.array_resource b <*> context))
-       f'
+    RST.rst_frame
+      R.(AR.array_resource b <*> context)
+      (fun _ -> R.(AR.array_resource b <*> context))
+      f'
   in
-  (**) assume(R.inv (R.(AR.array_resource b <*> context)) hinit);
-  (**) assume(RST.rst_inv (R.(AR.array_resource b <*> context)) hinit);
   (**) admit();
   L.for
     0ul
